WIP

Phi_System/Calculus_of_Programming.thy
@@ -43,7 +43,7 @@ consts programming_mode :: mode
        view_shift_mode  :: mode
 
 definition CurrentConstruction :: " mode \<Rightarrow> resource \<Rightarrow> assn \<Rightarrow> assn \<Rightarrow> bool "
-  where "CurrentConstruction mode s R S \<longleftrightarrow> s \<in> INTERP_SPEC (S * R)"
+  where "CurrentConstruction mode s R S \<longleftrightarrow> s \<Turnstile> INTERP_SPEC (S * R)"
 
 abbreviation Programming_CurrentConstruction ("(2\<c>\<u>\<r>\<r>\<e>\<n>\<t> _ [_] \<r>\<e>\<s>\<u>\<l>\<t>\<s> \<i>\<n>/ _)" [1000,1000,11] 10)
   where \<open>Programming_CurrentConstruction \<equiv> CurrentConstruction programming_mode\<close>
@@ -61,7 +61,8 @@ definition PendingConstruction :: " 'ret proc
                                   \<Rightarrow> (ABNM \<Rightarrow> assn)
                                   \<Rightarrow> bool "
     ("\<p>\<e>\<n>\<d>\<i>\<n>\<g> _ \<o>\<n> _ [_]/ \<r>\<e>\<s>\<u>\<l>\<t>\<s> \<i>\<n> _/ \<t>\<h>\<r>\<o>\<w>\<s> _" [1000,1000,1000,11,11] 10)
-    where "PendingConstruction f s R S E \<longleftrightarrow> f s \<subseteq> LooseState (\<lambda>ret. INTERP_SPEC (S ret * R)) (\<lambda>ex. INTERP_SPEC (E ex * R))"
+    where "PendingConstruction f s R S E \<longleftrightarrow>
+              BI_lift (f s) \<le> LooseState (\<lambda>ret. INTERP_SPEC (S ret * R)) (\<lambda>ex. INTERP_SPEC (E ex * R))"
 
 consts PendingConstruction_syntax :: \<open>'ret proc \<Rightarrow> ('ret \<phi>arg \<Rightarrow> assn) \<Rightarrow> (ABNM \<Rightarrow> assn) \<Rightarrow> bool\<close>
   ("\<p>\<e>\<n>\<d>\<i>\<n>\<g> \<p>\<r>\<o>\<c> _/ \<r>\<e>\<s>\<u>\<l>\<t>\<s> \<i>\<n> _/ \<t>\<h>\<r>\<o>\<w>\<s> _" [1000,11,11] 10)
@@ -124,7 +125,7 @@ lemma \<phi>assemble_proc:
   \<open> \<p>\<e>\<n>\<d>\<i>\<n>\<g> f \<o>\<n> s [R] \<r>\<e>\<s>\<u>\<l>\<t>\<s> \<i>\<n> T \<t>\<h>\<r>\<o>\<w>\<s> E1
 \<Longrightarrow> (\<And>s' ret. CodeBlock s s' f ret \<Longrightarrow> \<p>\<e>\<n>\<d>\<i>\<n>\<g> (g ret) \<o>\<n> s' [R] \<r>\<e>\<s>\<u>\<l>\<t>\<s> \<i>\<n> U \<t>\<h>\<r>\<o>\<w>\<s> E2)
 \<Longrightarrow> \<p>\<e>\<n>\<d>\<i>\<n>\<g> (f \<bind> g) \<o>\<n> s [R] \<r>\<e>\<s>\<u>\<l>\<t>\<s> \<i>\<n> U \<t>\<h>\<r>\<o>\<w>\<s> E1 + E2\<close>
-  unfolding CurrentConstruction_def PendingConstruction_def bind_def subset_iff CodeBlock_def
+  unfolding CurrentConstruction_def PendingConstruction_def bind_def less_eq_BI_iff CodeBlock_def
   apply clarsimp subgoal for s s'
   by (cases s; simp; cases s'; simp add: split_comp_All ring_distribs plus_fun) .
 
@@ -135,14 +136,13 @@ lemma \<phi>accept_proc:
   \<open> \<p>\<e>\<n>\<d>\<i>\<n>\<g> f \<o>\<n> s [R] \<r>\<e>\<s>\<u>\<l>\<t>\<s> \<i>\<n> T \<t>\<h>\<r>\<o>\<w>\<s> E
 \<Longrightarrow> CodeBlock s s' f ret
 \<Longrightarrow> \<c>\<u>\<r>\<r>\<e>\<n>\<t> s' [R] \<r>\<e>\<s>\<u>\<l>\<t>\<s> \<i>\<n> T ret\<close>
-  unfolding PendingConstruction_def bind_def subset_iff CurrentConstruction_def CodeBlock_def Satisfaction_def
+  unfolding PendingConstruction_def bind_def less_eq_BI_iff CurrentConstruction_def CodeBlock_def
   by blast
 
 lemma \<phi>accept_proc_optimize_return_v:
   \<open> \<p>\<e>\<n>\<d>\<i>\<n>\<g> (Return v) \<o>\<n> s [R] \<r>\<e>\<s>\<u>\<l>\<t>\<s> \<i>\<n> T \<t>\<h>\<r>\<o>\<w>\<s> E
 \<Longrightarrow> \<c>\<u>\<r>\<r>\<e>\<n>\<t> s [R] \<r>\<e>\<s>\<u>\<l>\<t>\<s> \<i>\<n> T v\<close>
-  unfolding PendingConstruction_def bind_def subset_iff CurrentConstruction_def Return_def
-            det_lift_def Satisfaction_def
+  unfolding PendingConstruction_def bind_def less_eq_BI_iff CurrentConstruction_def Return_def det_lift_def
   by simp
 
 
@@ -166,26 +166,26 @@ lemma \<phi>return_additional_unit:
 \<Longrightarrow> \<p>\<e>\<n>\<d>\<i>\<n>\<g> (f \<bind> (\<lambda>v. Return (\<phi>V_pair v \<phi>V_none))) \<o>\<n> s [R]
         \<r>\<e>\<s>\<u>\<l>\<t>\<s> \<i>\<n> (\<lambda>ret. T (\<phi>V_fst ret)) \<t>\<h>\<r>\<o>\<w>\<s> E\<close>
   unfolding CurrentConstruction_def PendingConstruction_def bind_def Return_def \<phi>V_pair_def
-    \<phi>V_fst_def \<phi>V_snd_def det_lift_def subset_iff
+    \<phi>V_fst_def \<phi>V_snd_def det_lift_def less_eq_BI_iff
   apply clarsimp subgoal for s' s'' by (cases s'; simp; cases s''; simp add: ring_distribs; blast) .
 
 lemma \<phi>return:
   " \<c>\<u>\<r>\<r>\<e>\<n>\<t> s [R] \<r>\<e>\<s>\<u>\<l>\<t>\<s> \<i>\<n> T'
 \<Longrightarrow> T' = T ret
 \<Longrightarrow> \<p>\<e>\<n>\<d>\<i>\<n>\<g> (Return ret) \<o>\<n> s [R] \<r>\<e>\<s>\<u>\<l>\<t>\<s> \<i>\<n> T \<t>\<h>\<r>\<o>\<w>\<s> 0"
-  unfolding CurrentConstruction_def PendingConstruction_def bind_def Return_def det_lift_def subset_iff Satisfaction_def
+  unfolding CurrentConstruction_def PendingConstruction_def bind_def Return_def det_lift_def less_eq_BI_iff
   by simp+
 
 lemma \<phi>reassemble_proc_final:
   "(\<And>s H. \<c>\<u>\<r>\<r>\<e>\<n>\<t> s [H] \<r>\<e>\<s>\<u>\<l>\<t>\<s> \<i>\<n> S \<Longrightarrow> \<p>\<e>\<n>\<d>\<i>\<n>\<g> g \<o>\<n> s [H] \<r>\<e>\<s>\<u>\<l>\<t>\<s> \<i>\<n> T \<t>\<h>\<r>\<o>\<w>\<s> E)
 \<Longrightarrow> \<p>\<r>\<o>\<c> g \<lbrace> S \<longmapsto> T \<rbrace> \<t>\<h>\<r>\<o>\<w>\<s> E"
-  unfolding CurrentConstruction_def PendingConstruction_def \<phi>Procedure_def bind_def split_paired_all Satisfaction_def
+  unfolding CurrentConstruction_def PendingConstruction_def \<phi>Procedure_def bind_def split_paired_all
   by (simp add: mult.commute)
 
 lemma "\<phi>__Return_rule__":
   \<open> X \<s>\<h>\<i>\<f>\<t>\<s> Y \<w>\<i>\<t>\<h> Any
 \<Longrightarrow> \<p>\<r>\<o>\<c> Return \<phi>V_none \<lbrace> X \<longmapsto> \<lambda>_::unit \<phi>arg. Y \<rbrace>\<close>
-  unfolding \<phi>Procedure_def Return_def View_Shift_def subset_iff det_lift_def Satisfaction_def
+  unfolding \<phi>Procedure_def Return_def View_Shift_def less_eq_BI_iff det_lift_def
   by clarsimp
 
 subsection \<open>Construct View Shift\<close>
@@ -193,8 +193,8 @@ subsection \<open>Construct View Shift\<close>
 lemma \<phi>make_view_shift:
   \<open> (\<And>s R. \<v>\<i>\<e>\<w> s [R] \<i>\<s> S \<Longrightarrow> (\<v>\<i>\<e>\<w> s [R] \<i>\<s> S' \<s>\<u>\<b>\<j> P))
 \<Longrightarrow> S \<s>\<h>\<i>\<f>\<t>\<s> S' \<w>\<i>\<t>\<h> P\<close>
-  unfolding CurrentConstruction_def View_Shift_def Satisfaction_def
-  by (simp add: INTERP_SPEC_subj Subjection_expn_set)
+  unfolding CurrentConstruction_def View_Shift_def
+  by (simp add: INTERP_SPEC_subj)
 
 
 subsection \<open>Construct Implication\<close>
@@ -210,7 +210,7 @@ lemma \<phi>apply_view_shift:
   " CurrentConstruction mode blk R S
 \<Longrightarrow> S \<s>\<h>\<i>\<f>\<t>\<s> S' \<w>\<i>\<t>\<h> P
 \<Longrightarrow> (CurrentConstruction mode blk R S') \<and> P"
-  unfolding CurrentConstruction_def View_Shift_def Satisfaction_def
+  unfolding CurrentConstruction_def View_Shift_def
   by (simp_all add: split_paired_all)
 
 lemmas \<phi>apply_implication = \<phi>apply_view_shift[OF _ view_shift_by_implication]
@@ -219,15 +219,15 @@ lemma \<phi>apply_view_shift_pending:
   " PendingConstruction f blk H T E
 \<Longrightarrow> (\<And>x. T x \<s>\<h>\<i>\<f>\<t>\<s> T' x \<w>\<i>\<t>\<h> P)
 \<Longrightarrow> PendingConstruction f blk H T' E"
-  unfolding PendingConstruction_def View_Shift_def Satisfaction_def
-  by (clarsimp simp add: LooseState_expn' subset_iff split_comp_All)
+  unfolding PendingConstruction_def View_Shift_def
+  by (clarsimp simp add: LooseState_expn' less_eq_BI_iff split_comp_All)
 
 lemma \<phi>apply_view_shift_pending_E:
   " PendingConstruction f blk H T E
 \<Longrightarrow> (\<And>x. E x \<s>\<h>\<i>\<f>\<t>\<s> E' x \<w>\<i>\<t>\<h> P)
 \<Longrightarrow> PendingConstruction f blk H T E'"
-  unfolding PendingConstruction_def View_Shift_def Satisfaction_def
-  by (clarsimp simp add: LooseState_expn' subset_iff split_comp_All)
+  unfolding PendingConstruction_def View_Shift_def
+  by (clarsimp simp add: LooseState_expn' less_eq_BI_iff split_comp_All)
 
 lemmas \<phi>apply_implication_pending =
   \<phi>apply_view_shift_pending[OF _ view_shift_by_implication]
@@ -354,7 +354,7 @@ paragraph \<open>Fact Store\<close>
 lemma [\<phi>programming_simps]:
   "CurrentConstruction mode s H (T \<s>\<u>\<b>\<j> P) \<longleftrightarrow> (CurrentConstruction mode s H T) \<and> P"
   unfolding CurrentConstruction_def
-  by (simp_all add: INTERP_SPEC_subj split_paired_all Subjection_expn_set)
+  by (simp_all add: INTERP_SPEC_subj split_paired_all)
 
 lemma [\<phi>programming_simps]:
   "(CurrentConstruction mode s H T \<and> B) \<and> C \<longleftrightarrow> (CurrentConstruction mode s H T) \<and> (B \<and> C)"
@@ -373,7 +373,7 @@ paragraph \<open>Fixing Existentially Quantified Variable\<close>
 lemma \<phi>ExTyp_strip:
   "(CurrentConstruction mode p H (\<exists>*c. T c)) \<equiv> (\<exists>c. CurrentConstruction mode p H (T c))"
   unfolding CurrentConstruction_def atomize_eq
-  by (simp_all add: INTERP_SPEC_ex split_paired_all Subjection_expn_set ExBI_expn_set)
+  by (simp_all add: INTERP_SPEC_ex split_paired_all)
 
 lemma \<phi>ExTyp_strip_imp:
   \<open>ToA_Construction s (\<exists>*c. T c) \<equiv> (\<exists>c. ToA_Construction s (T c))\<close>
@@ -423,19 +423,19 @@ lemma \<phi>M_Success[intro!]: (*deprecated?*)
   \<open> v \<Turnstile> (y \<Ztypecolon> T)
 \<Longrightarrow> \<p>\<r>\<o>\<c> Return (\<phi>arg v) \<lbrace> X \<longmapsto> \<lambda>u. y \<Ztypecolon> Val u T\<heavy_comma> X \<rbrace> \<t>\<h>\<r>\<o>\<w>\<s> Any \<close>
   unfolding \<phi>Procedure_def det_lift_def Return_def
-  by (clarsimp simp add: Val_def \<phi>Type_def)
+  by (clarsimp simp add: Val_def \<phi>Type_def less_eq_BI_iff)
 
 lemma \<phi>M_Success_P:
   \<open> v \<Turnstile> (y \<Ztypecolon> T)
 \<Longrightarrow> P (\<phi>arg v)
 \<Longrightarrow> \<p>\<r>\<o>\<c> Return (\<phi>arg v) \<lbrace> X \<longmapsto> \<lambda>u. y \<Ztypecolon> Val u T\<heavy_comma> X \<s>\<u>\<b>\<j> P u \<rbrace> \<t>\<h>\<r>\<o>\<w>\<s> Any \<close>
   unfolding \<phi>Procedure_def det_lift_def Return_def
-  by (clarsimp simp add: Val_def \<phi>Type_def INTERP_SPEC_subj Subjection_expn_set)
+  by (clarsimp simp add: Val_def \<phi>Type_def INTERP_SPEC_subj less_eq_BI_iff)
 
 declare \<phi>M_Success[where X=1, simplified, intro!]
 
 lemma \<phi>M_Success'[intro!]:
   \<open> \<p>\<r>\<o>\<c> Return vs \<lbrace> X vs \<longmapsto> X \<rbrace> \<t>\<h>\<r>\<o>\<w>\<s> Any \<close>
-  unfolding Return_def \<phi>Procedure_def det_lift_def by clarsimp
+  unfolding Return_def \<phi>Procedure_def det_lift_def less_eq_BI_iff by clarsimp
 
 end
